Added implementation of dynamic semantics for non-placement rules.

ReTierDynamicSemantics.v
@@ -1,4 +1,5 @@
 Require Import ReTierSyntax.
+Require Import Maps.
 Require Coq.Lists.ListSet.
 
 
@@ -69,3 +70,293 @@ Fixpoint subst_s (id: id) (value: t) (term: s): s :=
   end.
 
 Notation "[ id :=_s value ] term" := (subst_s id value term) (at level 40).
+
+
+Definition peerInsts := ListSet.set p.
+Definition noPeerInsts := ListSet.empty_set p.
+
+Definition eq_peerInstDec : forall x y : p, {x = y} + {x <> y}.
+  decide equality. decide equality.
+Defined.
+
+Definition pISet_add (x: p) (s: peerInsts): peerInsts :=
+  ListSet.set_add eq_peerInstDec x s.
+
+Definition pISet_mem (x: p) (s: peerInsts): bool :=
+  ListSet.set_mem eq_peerInstDec x s.
+
+
+
+
+Inductive reactiveSystem : Type :=
+  | ReactiveSystem: ListSet.set t -> partial_map t t -> reactiveSystem.
+
+Definition emptyReactSys := ReactiveSystem (ListSet.empty_set t) (p_empty t t).
+
+
+
+(** Context for local evaluation. **)
+Inductive leContext: Type :=
+  | LeContext: Ties -> peerTyping -> peerInsts -> P -> reactiveSystem-> leContext.
+
+Definition emptyLeContext := LeContext noTies noPeers noPeerInsts (Peer "_") emptyReactSys.
+
+
+Definition getPeerInstancesOfType (context: leContext) (PT: P): ListSet.set p :=
+    match context with
+    | LeContext _ typing insts _ _
+      =>  let hasTypePT (pInst: p): bool :=
+            match (typing pInst) with
+            | None => false
+            | Some PT2 => beq_peerType PT PT2
+            end
+          in Coq.Lists.List.filter hasTypePT insts
+    end.
+
+Definition getReactSys (context: leContext): reactiveSystem :=
+  match context with
+  | LeContext _ _ _ _ sys => sys
+  end.
+
+
+
+
+(* TODO: replace by lemma and prove it *)
+Hypothesis term_eq_dec : forall x y:t, {x = y} + {x <> y}.
+
+Definition reactDomainMem (x: t) (sys: reactiveSystem): bool :=
+  match sys with
+  | ReactiveSystem dom _ => ListSet.set_mem term_eq_dec x dom
+  end.
+
+Definition reactSysAdd (r val: t) (sys: reactiveSystem): reactiveSystem :=
+  match sys with
+  | ReactiveSystem dom map  => ReactiveSystem (ListSet.set_add term_eq_dec r dom)
+                                              (p_update beq_t map r val)
+  end.
+
+Definition reactGet (sys: reactiveSystem) (r: t): option t :=
+  match sys with
+  | ReactiveSystem _ map => map r
+  end.
+
+Inductive reactiveOp: Type :=
+  | allocSignal: t -> reactiveSystem -> reactiveOp
+  | allocVar: t -> reactiveSystem -> reactiveOp
+  | currentValue: t -> reactiveSystem -> reactiveOp
+  | updateVar: t -> t -> reactiveSystem -> reactiveOp.
+
+Reserved Notation "reactOp 'r=' '(' r ',' reactSys ')'" (at level 20).
+Inductive reactiveStep : reactiveOp -> t -> reactiveSystem -> Prop :=
+  | R_Signal: forall t rho r rho',
+        reactDomainMem r rho = false ->
+        rho' = reactSysAdd r t rho ->
+        allocSignal t rho r= (r, rho')
+  | R_Var: forall v rho r rho',
+        reactDomainMem r rho = false ->
+        rho' = reactSysAdd r v rho ->
+        allocVar v rho r= (r, rho')
+  | R_Retrieval: forall r rho t,
+        Some t = reactGet rho r ->
+        currentValue r rho r= (t, rho)
+  | R_Update: forall r v rho rho',
+        rho' = reactSysAdd r v rho ->
+        updateVar r v rho r= (unit, rho')
+
+where "reactOp 'r=' '(' r ',' reactSys ')'" := (reactiveStep reactOp r reactSys).
+
+
+(* ...just a little reminder
+  (** terms **)
+  Inductive t : Type :=
+    | lambda : id -> T -> t -> t
+    | app    : t -> t -> t
+    | idApp  : id -> t
+    | unit   : t
+    | none   : T -> t
+    | some   : t -> t
+    | nil    : T -> t
+    | cons   : t -> t -> t
+    | asLocal       : t -> S -> t
+    | asLocalFrom   : t -> S -> t -> t
+    | asLocalIn     : id -> t -> t -> S -> t
+    | asLocalInFrom : id -> t -> t -> S -> t -> t
+    | signal : t -> t
+    | var    : t -> t
+    | now    : t -> t
+    | set    : t -> t -> t
+    | peerApp          : p -> t
+    | remoteApp        : r -> t
+
+    (* Added to make testing easier. *)
+    | tnat   : nat -> t.
+*)
+Reserved Notation "'[' x ':=' s ']' tm" (at level 20).
+
+Fixpoint subst (x:id) (s tm: t): t :=
+  match tm with
+  | lambda y T body => if beq_id x y then lambda y T body else lambda y T (subst x s body)
+  | app f arg => app (subst x s f) (subst x s arg)
+  | idApp y   => if beq_id x y then s else (idApp y)
+  | unit      => unit
+  | none T    => none T
+  | some t    => some (subst x s t)
+  | nil T     => nil T
+  | cons t1 t2 => cons (subst x s t1) (subst x s t2)
+  | asLocal t (*:*) S => asLocal (subst x s t) (*:*) S
+  | asLocalFrom t1 (*:*) S (*from*) t2
+      => asLocalFrom (subst x s t1) (*:*) S (*from*) t2
+  | asLocalIn y (*=*) t1 (*in*) t2 (*:*) S
+      =>  if beq_id x y then asLocalIn y (*=*) (subst x s t1) (*in*) t2 (*:*) S
+          else asLocalIn y (*=*) (subst x s t1) (*in*) (subst x s t2) (*:*) S
+  | asLocalInFrom y (*=*) t1 (*in*) t2 (*:*) S (*from*) t3
+      =>  if beq_id x y
+          then asLocalInFrom y (*=*) (subst x s t1) (*in*) t2 (*:*) S (*from*) t3
+          else asLocalInFrom y (*=*) (subst x s t1) (*in*) (subst x s t2) (*:*) S (*from*) t3
+  | signal t => signal (subst x s t)
+  | var t => var (subst x s t)
+  | now t => now (subst x s t)
+  | set t1 t2 => set (subst x s t1) (subst x s t2)
+  | peerApp p => peerApp p
+  | remoteApp r => remoteApp r
+  | tnat n => tnat n    (*TODO: remove tnat *)
+  end
+where "'[' x ':=' s ']' tm" := (subst x s tm).
+
+
+
+
+(** Notation for local evaluation. **)
+(*Reserved Notation "context '|>' t1 'L==>' t2" (at level 40).*)
+Reserved Notation "context '|>' t1 'L==>' t2 ',' rho" (at level 45).
+
+(* TODO:  Let (LeContext insts PeerType pTyping) be the context given as first
+          argument for this Prop.
+          Check in all relevants rules if all elements of 'insts' have type
+          'PeerType' according to 'peerTyping'.
+*)
+(* TODO:  Add reactive context to Prop and rules. *)
+
+(* reminder
+  Inductive leContext: Type :=
+  | LeContext: peerTyping -> peerInsts -> P -> leContext.
+*)
+Inductive localStep : leContext -> t -> t -> reactiveSystem -> Prop :=
+  (* E_Context *)
+  | E_App: forall context x T t v,
+        context |> (app (lambda x T t) v) L==> [x := v] t, getReactSys context
+
+  (* remote access *)
+  | E_AsLocal: forall context peers ties P0 P1 v v' T _x _y _z,
+        context = LeContext ties _x _y P0 _z ->
+        peers = getPeerInstancesOfType context P1 ->
+        Some v' = Phi ties P0 P1 peers v T ->
+        context |> (asLocal v (*:*) (T on P1)) L==> v', getReactSys context
+
+  | E_Comp: forall context x v t T P1,
+        context |> (asLocalIn x (*=*) v (*in*) t (*:*) (T on P1))
+        L==> (asLocal ([x := v] t) (*:*) (T on P1)), getReactSys context
+
+  (* TODO: write tests *)
+  | E_Remote: forall context t t' T P1 context' ties typing peers P0 _x,
+        context = LeContext ties typing peers P0 _x ->
+        context' = LeContext ties typing peers P1 _x ->
+        context' |> t L==> t', getReactSys context  ->
+        context |> asLocal t (*:*) (T on P1) L==> asLocal t' (*:*) (T on P1), getReactSys context
+
+  | E_AsLocalFrom: forall context v T P1 p,
+        context |> asLocalFrom v (*:*) (T on P1) (*from*) p L==> v, getReactSys context
+
+  | E_CompFrom: forall context x v t S p,
+        context |> asLocalInFrom x (*=*) v (*in*) t (*:*) S (*from*) p
+        L==> asLocalFrom ([x := v] t) (*:*) S (*from*) p, getReactSys context
+
+  (* TODO: write tests *)
+  | E_RemoteFrom: forall context t t' T P1 p context' ties typing peers P0 _x,
+        context = LeContext ties typing peers P0 _x ->
+        context' = LeContext ties typing peers P1 _x ->
+        context' |> t L==> t', getReactSys context  ->
+        context |> asLocalFrom t (*:*) (T on P1) (*from*) p L==> asLocalFrom t' (*:*) (T on P1) (*from*) p, getReactSys context
+
+  (* reactive rules *)
+  | E_ReactiveVar: forall context v r rho rho' ,
+        rho = getReactSys context ->
+        (allocVar v rho) r= (r, rho') ->
+        context |> var v L==> r, getReactSys context
+
+  | E_Signal: forall context t r rho rho',
+        allocSignal t rho r= (r, rho') ->
+        context |> signal t L==> r, rho'
+
+  | E_Set: forall context r v rho rho',
+        updateVar r v rho r= (unit, rho') ->
+        context |> set r (*:=*) v L==> unit, rho'
+
+  | E_Now: forall context r t rho rho',
+        currentValue r rho r= (t, rho') ->
+        context |> now r L==> t, rho'
+
+where "context '|>' t1 'L==>' t2 ',' rho" := (localStep context t1 t2 (getReactSys context)).
+
+Notation "context '|>' t1 'L==>' t2" := (context |> t1 L==> t2, getReactSys context) (at level 40).
+
+
+Definition testTies1  :=  (tie_update (Peer "p0" *-> Peer "pm")
+                            (tie_update (Peer "p0" ?-> Peer "po")
+                              (tie_update (Peer "p0" S-> Peer "ps")
+                                (tie_update ((Peer "p0") N-> (Peer "pn"))
+                                  noTies)))).
+Definition testPeerTyping1 := (pT_update (PeerInst 4) (Peer "pm")
+                                (pT_update (PeerInst 3) (Peer "po")
+                                  (pT_update (PeerInst 2) (Peer "ps")
+                                    (pT_update (PeerInst 1) (Peer "pn")
+                                      (pT_update (PeerInst 0) (Peer "p0")
+                                      noPeers))))).
+Definition testPeerInsts1 := (pISet_add (PeerInst 4)
+                                (pISet_add (PeerInst 3)
+                                  (pISet_add (PeerInst 2)
+                                    (pISet_add (PeerInst 1)
+                                      (pISet_add (PeerInst 0)
+                                        noPeerInsts))))).
+Definition testTies1Context := LeContext testTies1 testPeerTyping1 testPeerInsts1 (Peer "p0") emptyReactSys.
+
+Example testLocalStep_EApp_1:
+  emptyLeContext |> (app (lambda (Id "x") (Option Unit) (unit)) (some unit)) L==> unit.
+Proof. apply E_App. Qed.
+
+Example testLocalStep_EApp_2:
+  emptyLeContext |> (app (lambda (Id "x") (Option Unit) (idApp (Id "x")))) (some unit) L==> (some unit).
+Proof. apply E_App. Qed.
+
+
+Example testLocalStep_EAsLocal_1:
+  testTies1Context |> (asLocal unit (*:*) (Unit on (Peer "ps"))) L==> unit.
+Proof.
+  eapply E_AsLocal.
+  - reflexivity.
+  - reflexivity.
+  - reflexivity.
+Qed.
+
+
+Example testLocalStep_EComp_1:
+  testTies1Context |> asLocalIn (Id "x") (*=*) unit (*in*)  (idApp (Id "x")) (*:*) (Unit on (Peer "ps"))
+  L==> asLocal unit (*:*) (Unit on (Peer "ps")).
+Proof. apply E_Comp. Qed.
+
+
+Example testLocalStep_EAsLocalFrom_1:
+  testTies1Context |> asLocalFrom unit (*:*) (Unit on (Peer "ps")) (*from*) (peerApp (PeerInst 2))
+  L==> unit.
+Proof. apply E_AsLocalFrom. Qed.
+
+
+Example testLocalStep_ECompFrom_1:
+  testTies1Context |> asLocalInFrom (Id "x") (*=*) unit (*in*) (idApp (Id "x")) (*:*) (Unit on (Peer "ps")) (*from*) (peerApp (PeerInst 2))
+  L==> asLocalFrom unit (*:*) (Unit on (Peer "ps")) (*from*) (peerApp (PeerInst 2)).
+Proof. apply E_CompFrom. Qed.
+
+
+
+
+
