ReTierSyntax.v
@@ -115,6 +115,11 @@ Proof. reflexivity. Qed.
 Example test_update_5: (idUpdate (Id "y") 2 (idUpdate (Id "x") 1 idEmpty) (Id "y")) = Some 2.
 Proof. reflexivity. Qed.
 
+Definition beq_r (a b: r): bool :=
+  match (a, b) with
+  | (remoteInst an, remoteInst bn) => Nat.eqb an bn
+  end.
+
 
 (** types **)
 Inductive T : Type :=
@@ -130,12 +135,29 @@ Inductive T : Type :=
 
 Notation "T1 ~> T2" := (Arrow T1 T2) (at level 80, right associativity).
 
+Fixpoint beq_T (a b: T): bool :=
+  match (a, b) with
+  | (a1 ~> a2, b1 ~> b2) => (beq_T a1 b1) && (beq_T a2 b2)
+  | (Unit, Unit) => true
+  | (Option a1, Option b1) => beq_T a1 b1
+  | (List a1, List b1) => beq_T a1 b1
+  | (Remote Pa, Remote Pb) => beq_peerType Pa Pb
+  | (Signal a1, Signal b1) => beq_T a1 b1
+  | (Var a1, Var b1) => beq_T a1 b1
+  | _ => false
+  end.
+
 
 (** placement types **)
 Inductive S : Type :=
   | on : T -> P -> S.
 
 Infix "on" := on (at level 20).
+
+Definition beq_S (a b: S): bool :=
+  match (a, b) with
+  | (aT on aP, bT on bP) => (beq_T aT bT) && (beq_peerType aP bP)
+  end.
 
 (** terms **)
 Inductive t : Type := 
@@ -161,6 +183,35 @@ Inductive t : Type :=
   (* Added to make testing easier. *)
   | tnat   : nat -> t.
 
+
+Fixpoint beq_t (a b: t): bool :=
+  match (a, b) with
+  | (lambda ax aT at_, lambda bx bT bt)
+      => (beq_id ax bx) && (beq_T aT bT) && (beq_t at_ bt)
+  | (app at1 at2, app bt1 bt2)    => (beq_t at1 bt1) && (beq_t at2 bt2)
+  | (idApp xa, idApp xb)          => beq_id xa xb
+  | (unit, unit)                  => true
+  | (none aT, none bT)            => beq_T aT bT
+  | (some at1, some bt1)          => beq_t at1 bt1
+  | (nil aT, nil bT)              => beq_T aT bT
+  | (cons at1 at2, cons bt1 bt2)  => (beq_t at1 bt1) && (beq_t at2 bt2)
+  | (asLocal at1 aS, asLocal bt1 bS) 
+      => (beq_t at1 bt1) && (beq_S aS bS)
+  | (asLocalFrom at1 aS at2, asLocalFrom bt1 bS bt2)
+      => (beq_t at1 bt1) && (beq_S aS bS) && (beq_t at2 bt2)
+  | (asLocalIn ax at1 at2 aS, asLocalIn bx bt1 bt2 bS)
+      => (beq_id ax bx) && (beq_t at1 at2) && (beq_t at2 bt2) && (beq_S aS bS)
+  | (asLocalInFrom ax at1 at2 aS at3, asLocalInFrom bx bt1 bt2 bS bt3)
+      => (beq_id ax bx) && (beq_t at1 at2) && (beq_t at2 bt2) && (beq_S aS bS) && (beq_t at3 bt3)
+  | (signal at1, signal bt1)      => beq_t at1 bt1
+  | (var at1, var bt1)            => beq_t at1 bt1
+  | (now at1, now bt1)            => beq_t at1 bt1
+  | (set at1 at2, set bt1 bt2)    => (beq_t at1 bt1) && (beq_t at2 bt2)
+  | (peerApp ap, peerApp bp)      => beq_peerInst ap bp
+  | (remoteApp ar, remoteApp br)  => beq_r ar br
+  | (tnat an, tnat bn)            => Nat.eqb an bn
+  | _                             => false
+  end.
 
 (*
 Notation "\ x ; T , t" := (lambda (Id x) T t) (at level 80, left associativity).
